more progress on defining refinements

Refinement.v
@@ -5,6 +5,7 @@ Add LoadPath "." as Specware.
 Require Import Specware.Util.
 Require Export Specware.Base.
 
+Import ListNotations.
 Require Export Coq.Logic.Eqdep.
 
 
@@ -35,53 +36,183 @@ Definition id_refinement {flds} spec : Refinement (flds:=flds) spec :=
 Ltac end_refine := apply id_refinement.
 
 
-(*** A Refinement step that applies an arbitrary morphism ***)
+(*** A Refinement step that applies a morphism ***)
 
 (* Applying a morphism to prove a refinement goal *)
-Definition apply_morphism_fun {flds1} (spec1 : Spec (flds:=flds1))
-           {flds2} (spec2 : Spec (flds:=flds2))
+Definition apply_morphism_fun {flds1} {spec1 : Spec (flds:=flds1)}
+           {flds2} {spec2 : Spec (flds:=flds2)}
            (m12 : Morphism spec1 spec2) :
   Refinement spec2 ->
   Refinement spec1.
   intro ref2; destruct ref2 as [ flds3 spec3 m23 ].
   apply (mkRefinement _ spec3);
   apply (mcompose m12 m23).
+Defined.
+
+(* The above as a tactic, so we don't have to write "apply apply_morphism" *)
+Ltac apply_morphism morph := apply (apply_morphism_fun morph).
+
+
+(*** Refinement of sub-specs ***)
+
+Definition IsMorphism_ConsNone f A {flds1} spec1 {flds2} spec2 m :
+  (forall a, @IsMorphism flds1 (spec1 a) flds2 (spec2 a) m) ->
+  IsMorphism (Spec_ConsNone f A spec1) (Spec_ConsNone (applyFM m f) A spec2) m.
+  intros ismorph model ism.
+  destruct ism as [ a sig ]; destruct sig as [ melem ism ].
+  exists a; split; [ | apply ismorph ]; assumption.
 Qed.
 
-(* the tactic version; mostly used by other tactics *)
-Ltac apply_morphism morph :=
-  apply (apply_morphism_fun _ _ morph).
+Definition IsMorphism_ConsSome f A a {flds1} spec1 {flds2} spec2 m :
+  @IsMorphism flds1 spec1 flds2 spec2 m ->
+  IsMorphism (Spec_ConsSome f A a spec1) (Spec_ConsSome (applyFM m f) A a spec2) m.
+  intros ismorph model ism.
+  destruct ism as [ melem ism ]; split; [ | apply ismorph ]; assumption.
+Qed.
 
 
 (*** Instantiating a field in a spec ***)
 
-Lemma IsModel_SomeToNone f A a {flds} (spec : A -> Spec (flds:=flds)) model :
-  IsModel model ({# f ::: A := a ; spec a #}) ->
-  IsModel model ({# f ::: A ;  x =>  spec x #}).
-  intro ism; destruct ism.
-  exists a; split; assumption.
+Lemma IsMorphism_instantiate_base f A a {flds} (spec : A -> Spec (flds:=flds)) :
+  IsMorphism (Spec_ConsNone f A spec) (Spec_ConsSome f A a (spec a)) idFM.
+  intros model ism; destruct ism.
+  exists a; split;
+  [ rewrite idFM_is_id | rewrite spec_map_id ]; assumption.
 Qed.
 
+Definition instantiate_field_base f {A} (a:A) {flds} (spec : A -> @Spec flds) :
+  { spec' : @Spec (f :: flds) | IsMorphism (Spec_ConsNone f A spec) spec' idFM } :=
+  existT _ (Spec_ConsSome f A a (spec a)) (IsMorphism_instantiate_base _ _ _ _).
+
 (*
-Definition instantiate_helper_base_fun
-        f A a {flds} (spec : A -> Spec (flds:=flds)) :
-  { spec' : Spec (flds:= f :: flds) & IsMorphism (Spec_ConsNone f A spec) spec' idFM } :=
-  existT (fun spec' => IsMorphism _ spec' id) (Spec_ConsSome f A a (spec a))
-         (fun model2 ism2 =>
-            existT2 (fun _ => _) (fun _ => _) model2
-                    (IsModel_SomeToNone _ _ _ _ _ ism2)
-                    (SuperModel_map_id _)).
+Definition instantiate_field_base f A a {flds} {spec : A -> Spec (flds:=flds)} :
+  Refinement (Spec_ConsSome f A a (spec a)) ->
+  Refinement (Spec_ConsNone f A spec) :=
+  apply_morphism_fun (mkMorphism _ _ idFM (IsMorphism_instantiate_base _ _ _ _)).
 *)
 
-Lemma IsMorphism_id_ConsNone f A {flds} (spec1 : A -> Spec (flds:=flds))
+Lemma IsMorphism_instantiate_ConsNone f A {flds} (spec1 : A -> Spec (flds:=flds))
       (spec2 : A -> Spec (flds:=flds)) :
   (forall a, IsMorphism (spec1 a) (spec2 a) idFM) ->
-  IsMorphism ({# f ::: A ; a => spec1 a #}) ({# f ::: A ; a => spec2 a #}) idFM.
+  IsMorphism (Spec_ConsNone f A spec1) (Spec_ConsNone f A spec2) idFM.
   intros ismorph model ism;
   destruct ism as [ a sig ]; destruct sig as [ melem ism ].
   exists a; split;
-  [ rewrite idFM_is_id; assumption | apply ismorph; assumption ].
+  [ rewrite idFM_is_id | apply ismorph ]; assumption.
 Qed.
+
+Definition instantiate_field_None f A {flds} {spec : A -> @Spec flds}
+  (fn : forall a, { spec' : @Spec flds |
+                    IsMorphism (spec a) spec' idFM }) :
+  { spec' : @Spec (f :: flds) | IsMorphism (Spec_ConsNone f A spec) spec' idFM } :=
+  existT _ (Spec_ConsNone f A (fun a => projT1 (fn a)))
+         (IsMorphism_instantiate_ConsNone
+            f A spec _
+            (fun a => projT2 (fn a))).
+
+Lemma IsMorphism_instantiate_ConsSome f A a {flds} (spec1 : Spec (flds:=flds))
+      (spec2 : Spec (flds:=flds)) :
+  IsMorphism spec1 spec2 idFM ->
+  IsMorphism (Spec_ConsSome f A a spec1) (Spec_ConsSome f A a spec2) idFM.
+  intros ismorph model ism;
+  destruct ism as [ melem ism ].
+  split; [ rewrite idFM_is_id | apply ismorph ]; assumption.
+Qed.
+
+Definition instantiate_field_Some f A a {flds} {spec : @Spec flds}
+  (rest : { spec' : @Spec flds | IsMorphism spec spec' idFM }) :
+  { spec' : @Spec (f :: flds) | IsMorphism (Spec_ConsSome f A a spec) spec' idFM } :=
+  existT _ (Spec_ConsSome f A a (projT1 rest))
+         (IsMorphism_instantiate_ConsSome f A a spec _ (projT2 rest)).
+
+
+(* A helper tactic which repeatedly tries to apply instantiate_field_* above *)
+Ltac instantiate_helper f val :=
+  repeat (apply (instantiate_field_base f val) ||
+          apply instantiate_field_None ||
+          apply instantiate_field_Some).
+
+FIXME HERE: figure out how to write this stupid tactic!
+
+(* The tactic itself *)
+Ltac instantiate_field f val :=
+  match goal with
+    | |- @Refinement ?flds ?spec =>
+      let H := fresh "H" in
+      let spec' := fresh "spec" in
+      let ism := fresh "isMorph" in
+      assert ({ spec' : @Spec flds | IsMorphism spec spec' id }) as H;
+        [ instantiate_helper f val | ];
+      destruct H as [ spec' ism ];
+      apply_morphism (mkMorphism spec spec' id ism)
+    | _ => fail "Not a refinement goal!"
+  end.
+
+Definition test_spec_fun :=
+  Spec_ConsNone "T" Set (fun T =>
+  Spec_ConsNone "f" (T -> T) (fun f =>
+  Spec_Nil)).
+
+(* Set Ltac Debug. *)
+
+Definition test_spec_id : Refinement test_spec_fun.
+  assert ({ spec' : @Spec ["T"%string; "f"%string ] | IsMorphism test_spec_fun spec' idFM }) as H.
+  instantiate_helper ("T"%string) (fun (x:nat) => x).
+
+  instantiate_field ("f"%string) (fun T (x:T) => x).
+
+Eval compute in (get_fields test_spec_fun).
+
+Definition test_spec_id : Refinement test_spec_fun.
+  assert ({ spec' : @Spec ["T"%string; "f"%string ] | IsMorphism test_spec_fun spec' idFM }) as H.
+  apply instantiate_field_None; intro a.
+  apply (instantiate_field_base (fun x => x)).
+  destruct H as [ spec' ismorph ]; apply_morphism (mkMorphism _ _ _ ismorph).
+  end_refine.
+Defined.
+
+Eval compute in (refinementSpec test_spec_id).
+
+
+
+Definition test_spec_id :=
+  Spec_ConsNone "T" Set (fun T =>
+  Spec_ConsSome "idT" (T -> T) (fun t => t)
+  Spec_Nil).
+
+Definition test_spec_id_nat :=
+  Spec_ConsSome "T" Set nat (
+  Spec_ConsSome "idT" (nat -> nat) (fun t => t)
+  Spec_Nil).
+
+(* FIXME: cannot get type-class resolution to work here... *)
+(*
+Section instantiation.
+
+  Class InstantiatesTo
+        {flds1} (spec1 : Spec (flds:=flds1))
+        {flds2} (spec2 : Spec (flds:=flds2)) : Prop :=
+    instantiation_ismorph_id : IsMorphism spec1 spec2 idFM.
+
+  Variables (flds:list string) (fld:string) (A:Type) (a:A)
+            (spec:A -> Spec (flds:=flds)).
+
+  Global Instance InstantiatesTo_Base :
+    InstantiatesTo (Spec_ConsNone fld A spec) (Spec_ConsSome fld A a (spec a)).
+  intros model ism; destruct ism.
+  exists a; split;
+  [ rewrite idFM_is_id | rewrite spec_map_id ]; assumption.
+  Qed.
+
+  (*
+  Definition test1 :
+    InstantiatesTo (Spec_ConsNone fld A spec) (Spec_ConsSome fld A a (spec a))
+    := instantiation_ismorph_id.
+   *)
+
+End instantiation.
+*)
+
 
 (*
 Program Definition instantiate_helper_step_ConsNone
